src/StepSeq.v
@@ -2,34 +2,36 @@ Require Import Bool List String Peano_dec.
 Require Import Permutation.
 Require Import Common FMap Syntax Semantics StepDet Serial.
 
-Record ATState : Type :=
-  { atst_oss : ObjectStates;
-    atst_msgs : Messages TMsg;
-    atst_tid : TrsId;
-    atst_cur : TrsId
-  }.
+(* Record ATState : Type := *)
+(*   { atst_oss : ObjectStates; *)
+(*     atst_msgs : Messages TMsg; *)
+(*     atst_tid : TrsId; *)
+(*     atst_cur : TrsId *)
+(*   }. *)
 
-Definition getATStateInit (sys: System): ATState :=
-  {| atst_oss := getObjectStatesInit (sys_objs sys);
-     atst_msgs := [];
-     atst_tid := trsIdInit;
-     atst_cur := trsIdInit
-  |}.
+(* Definition getATStateInit (sys: System): ATState := *)
+(*   {| atst_oss := getObjectStatesInit (sys_objs sys); *)
+(*      atst_msgs := []; *)
+(*      atst_tid := trsIdInit; *)
+(*      atst_cur := trsIdInit *)
+(*   |}. *)
 
-Instance ATState_HasInit: HasInit ATState :=
-  { getStateInit := getATStateInit }.
+(* Instance ATState_HasInit: HasInit ATState := *)
+(*   { getStateInit := getATStateInit }. *)
 
-Definition at2TState (ats: ATState) :=
-  {| tst_oss := atst_oss ats;
-     tst_msgs := atst_msgs ats;
-     tst_tid := atst_tid ats |}.
+(* Definition at2TState (ats: ATState) := *)
+(*   {| tst_oss := atst_oss ats; *)
+(*      tst_msgs := atst_msgs ats; *)
+(*      tst_tid := atst_tid ats |}. *)
 
-Inductive step_seq (sys: System) : ATState -> TLabel -> ATState -> Prop :=
+Inductive step_seq (sys: System) : TState -> TLabel -> TState -> Prop :=
 | SsSlt: forall st, step_seq sys st emptyILabel st
-| SsInt: forall ts cts oss oims obj idx os pos (fmsg: TMsg) fpmsg fidx fchn outs,
+| SsInt: forall ts oss oims obj idx os pos (fmsg: TMsg) fpmsg fidx fchn outs,
     In obj (sys_objs sys) ->
     idx = obj_idx obj ->
     oss@[idx] = Some os ->
+
+    isInternal sys (mid_from (msg_id (getMsg fmsg))) = true ->
 
     firstM fidx idx fchn oims = Some fmsg -> 
     msg_id (getMsg fmsg) = pmsg_mid fpmsg ->
@@ -44,22 +46,19 @@ Inductive step_seq (sys: System) : ATState -> TLabel -> ATState -> Prop :=
     tmsg_tid fmsg = ts ->
 
     step_seq sys
-             {| atst_oss := oss;
-                atst_msgs := oims;
-                atst_tid := ts;
-                atst_cur := cts |}
+             {| tst_oss := oss;
+                tst_msgs := oims;
+                tst_tid := ts |}
              (IlblInt (Some fmsg) (extOuts sys (toTMsgs (tmsg_tid fmsg) outs)))
-             {| atst_oss := oss +[ idx <- pos ];
-                atst_msgs := distributeMsgs (intOuts sys (toTMsgs (tmsg_tid fmsg) outs)) oims;
-                atst_tid := ts;
-                atst_cur := cts |}
+             {| tst_oss := oss +[ idx <- pos ];
+                tst_msgs := distributeMsgs (intOuts sys (toTMsgs (tmsg_tid fmsg) outs)) oims;
+                tst_tid := ts |}
 
-| SsExt: forall ts cts nts (Hts: nts > ts) oss oims obj os pos (emsg: Msg) fpmsg outs,
+| SsExt: forall ts nts (Hts: nts > ts) oss oims obj os pos (emsg: Msg) fpmsg outs,
     In obj (sys_objs sys) ->
     oss@[obj_idx obj] = Some os ->
 
     isExternal sys (mid_from (msg_id emsg)) = true ->
-    isInternal sys (mid_to (msg_id emsg)) = true ->
 
     msg_id emsg = pmsg_mid fpmsg ->
     In fpmsg (obj_trs obj) ->
@@ -69,13 +68,11 @@ Inductive step_seq (sys: System) : ATState -> TLabel -> ATState -> Prop :=
     ValidOuts (obj_idx obj) outs ->
 
     step_seq sys
-             {| atst_oss := oss;
-                atst_msgs := oims;
-                atst_tid := ts;
-                atst_cur := cts |}
-             (IlblExt {| tmsg_msg := emsg; tmsg_tid := ts |} (extOuts sys (toTMsgs ts outs)))
-             {| atst_oss := oss +[ obj_idx obj <- pos ];
-                atst_msgs := distributeMsgs (intOuts sys (toTMsgs ts outs)) oims;
-                atst_tid := nts;
-                atst_cur := nts |}.
+             {| tst_oss := oss;
+                tst_msgs := oims;
+                tst_tid := ts |}
+             (IlblExt {| tmsg_msg := emsg; tmsg_tid := nts |} (extOuts sys (toTMsgs nts outs)))
+             {| tst_oss := oss +[ obj_idx obj <- pos ];
+                tst_msgs := distributeMsgs (intOuts sys (toTMsgs ts outs)) oims;
+                tst_tid := nts |}.
 
