src/StepDet.v
@@ -3,46 +3,49 @@ Require Import Common FMap Syntax Semantics.
 
 Inductive step_det (sys: System) : TState -> TLabel -> TState -> Prop :=
 | SdSlt: forall st, step_det sys st emptyILabel st
-| SdInt: forall ts oss oims obj idx os pos (fmsg: TMsg) fpmsg fidx fchn outs,
+| SdInt: forall ts oss oims obj oidx os pos (fmsg: TMsg) fpmsg fidx fchn outs,
     In obj (sys_objs sys) ->
-    idx = obj_idx obj ->
-    oss@[idx] = Some os ->
+    oidx = obj_idx obj ->
+    oss@[oidx] = Some os ->
 
-    firstM fidx idx fchn oims = Some fmsg -> 
+    isInternal sys (mid_from (msg_id (getMsg fmsg))) = true ->
+
+    ValidMsgId fidx oidx fchn fmsg ->
+    firstM fidx oidx fchn oims = Some fmsg -> 
+
     msg_id (getMsg fmsg) = pmsg_mid fpmsg ->
-    ValidMsgId fidx idx fchn fmsg ->
     In fpmsg (obj_trs obj) ->
     pmsg_precond fpmsg os ->
     pmsg_postcond fpmsg os (msg_value (getMsg fmsg)) pos ->
     outs = pmsg_outs fpmsg os (msg_value (getMsg fmsg)) ->
-    ValidOuts (obj_idx obj) outs ->
+    ValidOuts oidx outs ->
 
     step_det sys
              {| tst_oss := oss; tst_msgs := oims; tst_tid := ts |}
              (IlblInt (Some fmsg) (extOuts sys (toTMsgs (tmsg_tid fmsg) outs)))
-             {| tst_oss := oss +[ idx <- pos ];
+             {| tst_oss := oss +[ oidx <- pos ];
                 tst_msgs := distributeMsgs (intOuts sys (toTMsgs (tmsg_tid fmsg) outs)) oims;
                 tst_tid := ts
              |}
 
-| SdExt: forall ts nts (Hts: nts > ts) oss oims obj os pos (emsg: Msg) fpmsg outs,
+| SdExt: forall ts nts (Hts: nts > ts) oss oims obj oidx os pos (emsg: Msg) fpmsg outs,
     In obj (sys_objs sys) ->
-    oss@[obj_idx obj] = Some os ->
+    oidx = obj_idx obj ->
+    oss@[oidx] = Some os ->
 
     isExternal sys (mid_from (msg_id emsg)) = true ->
-    isInternal sys (mid_to (msg_id emsg)) = true ->
 
     msg_id emsg = pmsg_mid fpmsg ->
     In fpmsg (obj_trs obj) ->
     pmsg_precond fpmsg os ->
     pmsg_postcond fpmsg os (msg_value emsg) pos ->
     outs = pmsg_outs fpmsg os (msg_value emsg) ->
-    ValidOuts (obj_idx obj) outs ->
+    ValidOuts oidx outs ->
 
     step_det sys
              {| tst_oss := oss; tst_msgs := oims; tst_tid := ts |}
-             (IlblExt {| tmsg_msg := emsg; tmsg_tid := ts |} (extOuts sys (toTMsgs ts outs)))
-             {| tst_oss := oss +[ obj_idx obj <- pos ];
+             (IlblExt {| tmsg_msg := emsg; tmsg_tid := nts |} (extOuts sys (toTMsgs nts outs)))
+             {| tst_oss := oss +[ oidx <- pos ];
                 tst_msgs := distributeMsgs (intOuts sys (toTMsgs ts outs)) oims;
                 tst_tid := nts
              |}.
